src/ReactorModel/Determinism/Dependency.lean
@@ -13,10 +13,9 @@ notation:50 rcn₁ " ≮[" rtr "] " rcn₂ => Independent rtr rcn₁ rcn₂
 variable {rtr : Reactor} {rcn₁ rcn₂ : ID} 
 variable (m₁ : rcn₁ ∈ rtr[.rcn]) (m₂ : rcn₂ ∈ rtr[.rcn]) (hi : rcn₁ ≮[rtr] rcn₂)
 
-theorem nonoverlapping_deps : rtr⟦m₁⟧.deps .out ∩ rtr⟦m₂⟧.deps .in = ∅ := by
-  have := hi
-  sorry -- exact absurd (ReactorType.Dependency.depOverlap ho₁ ho₂ $ Finset.nonempty_of_ne_empty hc) hi
- 
+theorem deps_disjoint : Disjoint (rtr⟦m₁⟧.deps .out) (rtr⟦m₂⟧.deps .in) := 
+  byContradiction fun hd => absurd (ReactorType.Dependency.depOverlap m₁ m₂ hd) hi
+
 theorem ne_con_or_pure (hn : rcn₁ ≠ rcn₂) : 
     (rtr⟦m₁⟧&.id ≠ rtr⟦m₂⟧&.id) ∨ rtr⟦m₁⟧.Pure ∨ rtr⟦m₂⟧.Pure := by
   have := hi
